more work on intLangExtraTheory
up to Cevaluate_syneq

compiler/proofs/intLangExtraScript.sml
@@ -303,10 +303,13 @@ val Cevaluate_vlabs = store_thm("Cevaluate_vlabs",
   strip_tac >- ( srw_tac[DNF_ss][SUBSET_DEF] >> metis_tac[] ) >>
   strip_tac >- ( srw_tac[DNF_ss][SUBSET_DEF] >> metis_tac[] ))
 
+val no_vlabs_menv_def = Define`no_vlabs_menv menv = ∀env. env ∈ (FRANGE menv) ⇒ no_vlabs_list env`
+val all_vlabs_menv_def = Define`all_vlabs_menv menv = ∀env. env ∈ (FRANGE menv) ⇒ all_vlabs_list env`
+
 val Cevaluate_no_vlabs = store_thm("Cevaluate_no_vlabs",
-  ``(∀menv s env exp res. Cevaluate menv s env exp res ⇒ no_vlabs_list s ∧ no_vlabs_list env ∧ no_labs exp ⇒
+  ``(∀menv s env exp res. Cevaluate menv s env exp res ⇒ no_vlabs_menv menv ∧ no_vlabs_list s ∧ no_vlabs_list env ∧ no_labs exp ⇒
         no_vlabs_list (FST res) ∧ (∀v. (SND res = Cval v) ⇒ no_vlabs v) ∧ (∀v. (SND res = Cexc (Craise v)) ⇒ no_vlabs v)) ∧
-    (∀menv s env es res. Cevaluate_list menv s env es res ⇒ no_vlabs_list s ∧ no_vlabs_list env ∧ no_labs_list es ⇒
+    (∀menv s env es res. Cevaluate_list menv s env es res ⇒ no_vlabs_menv menv ∧ no_vlabs_list s ∧ no_vlabs_list env ∧ no_labs_list es ⇒
         no_vlabs_list (FST res) ∧ (∀vs. (SND res = Cval vs) ⇒ no_vlabs_list vs) ∧ (∀v. (SND res = Cexc (Craise v)) ⇒ no_vlabs v))``,
   ho_match_mp_tac Cevaluate_ind >>
   strip_tac >- fsrw_tac[DNF_ss][EVERY_MEM,MEM_EL] >>
@@ -315,6 +318,7 @@ val Cevaluate_no_vlabs = store_thm("Cevaluate_no_vlabs",
   strip_tac >- simp[] >>
   strip_tac >- simp[] >>
   strip_tac >- fsrw_tac[DNF_ss][EVERY_MEM,MEM_EL] >>
+  strip_tac >- fsrw_tac[DNF_ss][EVERY_MEM,MEM_EL,IN_FRANGE,FLOOKUP_DEF,no_vlabs_menv_def] >>
   strip_tac >- fsrw_tac[DNF_ss][EVERY_MEM,MEM_EL] >>
   strip_tac >- fsrw_tac[DNF_ss][EVERY_MEM,MEM_EL] >>
   strip_tac >- fsrw_tac[DNF_ss][EVERY_MEM,MEM_EL] >>
@@ -338,7 +342,7 @@ val Cevaluate_no_vlabs = store_thm("Cevaluate_no_vlabs",
   strip_tac >- fsrw_tac[DNF_ss][EVERY_MEM,MEM_EL] >>
   strip_tac >- fsrw_tac[DNF_ss][EVERY_MEM,MEM_EL] >>
   strip_tac >- (
-    ntac 2 gen_tac >>
+    ntac 3 gen_tac >>
     Cases >> ntac 2 gen_tac >>
     Cases >> rw[] >>
     fs[el_check_def,EVERY_MEM] >>
@@ -347,19 +351,19 @@ val Cevaluate_no_vlabs = store_thm("Cevaluate_no_vlabs",
     metis_tac[MEM_EL]) >>
   strip_tac >- fsrw_tac[DNF_ss][EVERY_MEM,MEM_EL] >>
   strip_tac >- (
-    ntac 2 gen_tac >>
+    ntac 3 gen_tac >>
     Cases >> ntac 3 gen_tac >>
     Cases >> TRY (Cases_on`l`) >> Cases >> TRY (Cases_on`l`) >> rw[] ) >>
   strip_tac >- rw[] >>
   strip_tac >- (
-    ntac 5 gen_tac >>
+    ntac 6 gen_tac >>
     Cases >> rw[] >> fs[] >>
     fs[EVERY_MEM] >>
     fsrw_tac[DNF_ss][EVERY_MEM] >>
     metis_tac[MEM_LUPDATE] ) >>
   strip_tac >- fsrw_tac[DNF_ss][EVERY_MEM,MEM_EL] >>
   strip_tac >- (
-    ntac 6 gen_tac >>
+    ntac 7 gen_tac >>
     Cases >> fsrw_tac[DNF_ss][EVERY_MEM,MEM_EL] ) >>
   strip_tac >- fsrw_tac[DNF_ss][EVERY_MEM,MEM_EL] >>
   strip_tac >- fsrw_tac[DNF_ss][EVERY_MEM,MEM_EL] >>
@@ -368,9 +372,9 @@ val Cevaluate_no_vlabs = store_thm("Cevaluate_no_vlabs",
   strip_tac >- fsrw_tac[DNF_ss][EVERY_MEM,MEM_EL])
 
 val Cevaluate_all_vlabs = store_thm("Cevaluate_all_vlabs",
-  ``(∀s env exp res. Cevaluate s env exp res ⇒ all_vlabs_list s ∧ all_vlabs_list env ∧ all_labs exp ⇒
+  ``(∀menv s env exp res. Cevaluate menv s env exp res ⇒ all_vlabs_menv menv ∧ all_vlabs_list s ∧ all_vlabs_list env ∧ all_labs exp ⇒
         all_vlabs_list (FST res) ∧ (∀v. (SND res = Cval v) ⇒ all_vlabs v) ∧ (∀v. (SND res = Cexc (Craise v)) ⇒ all_vlabs v)) ∧
-    (∀s env es res. Cevaluate_list s env es res ⇒ all_vlabs_list s ∧ all_vlabs_list env ∧ all_labs_list es ⇒
+    (∀menv s env es res. Cevaluate_list menv s env es res ⇒ all_vlabs_menv menv ∧ all_vlabs_list s ∧ all_vlabs_list env ∧ all_labs_list es ⇒
         all_vlabs_list (FST res) ∧ (∀vs. (SND res = Cval vs) ⇒ all_vlabs_list vs) ∧ (∀v. (SND res = Cexc (Craise v)) ⇒ all_vlabs v))``,
   ho_match_mp_tac Cevaluate_ind >>
   strip_tac >- fsrw_tac[DNF_ss][EVERY_MEM,MEM_EL] >>
@@ -379,6 +383,7 @@ val Cevaluate_all_vlabs = store_thm("Cevaluate_all_vlabs",
   strip_tac >- simp[] >>
   strip_tac >- simp[] >>
   strip_tac >- fsrw_tac[DNF_ss][EVERY_MEM,MEM_EL] >>
+  strip_tac >- fsrw_tac[DNF_ss][EVERY_MEM,MEM_EL,IN_FRANGE,FLOOKUP_DEF,all_vlabs_menv_def] >>
   strip_tac >- fsrw_tac[DNF_ss][EVERY_MEM,MEM_EL] >>
   strip_tac >- fsrw_tac[DNF_ss][EVERY_MEM,MEM_EL] >>
   strip_tac >- fsrw_tac[DNF_ss][EVERY_MEM,MEM_EL] >>
@@ -402,7 +407,7 @@ val Cevaluate_all_vlabs = store_thm("Cevaluate_all_vlabs",
   strip_tac >- fsrw_tac[DNF_ss][EVERY_MEM,MEM_EL] >>
   strip_tac >- fsrw_tac[DNF_ss][EVERY_MEM,MEM_EL] >>
   strip_tac >- (
-    ntac 2 gen_tac >>
+    ntac 3 gen_tac >>
     Cases >> ntac 2 gen_tac >>
     Cases >> rw[] >>
     fs[el_check_def,EVERY_MEM] >>
@@ -411,19 +416,19 @@ val Cevaluate_all_vlabs = store_thm("Cevaluate_all_vlabs",
     metis_tac[MEM_EL]) >>
   strip_tac >- fsrw_tac[DNF_ss][EVERY_MEM,MEM_EL] >>
   strip_tac >- (
-    ntac 2 gen_tac >>
+    ntac 3 gen_tac >>
     Cases >> ntac 3 gen_tac >>
     Cases >> TRY (Cases_on`l`) >> Cases >> TRY (Cases_on`l`) >> rw[] ) >>
   strip_tac >- rw[] >>
   strip_tac >- (
-    ntac 5 gen_tac >>
+    ntac 6 gen_tac >>
     Cases >> rw[] >> fs[] >>
     fs[EVERY_MEM] >>
     fsrw_tac[DNF_ss][EVERY_MEM] >>
     metis_tac[MEM_LUPDATE] ) >>
   strip_tac >- fsrw_tac[DNF_ss][EVERY_MEM,MEM_EL] >>
   strip_tac >- (
-    ntac 6 gen_tac >>
+    ntac 7 gen_tac >>
     Cases >> fsrw_tac[DNF_ss][EVERY_MEM,MEM_EL] ) >>
   strip_tac >- fsrw_tac[DNF_ss][EVERY_MEM,MEM_EL] >>
   strip_tac >- fsrw_tac[DNF_ss][EVERY_MEM,MEM_EL] >>
@@ -550,43 +555,43 @@ val _ = export_rewrites["Cmap_result_def"]
 
 val Cevaluate_lit = store_thm(
 "Cevaluate_lit",
-``∀s env l res. Cevaluate s env (CLit l) res = (res = (s, Cval (CLitv l)))``,
+``∀menv s env l res. Cevaluate menv s env (CLit l) res = (res = (s, Cval (CLitv l)))``,
 rw[Once Cevaluate_cases])
 
 val Cevaluate_var = store_thm(
 "Cevaluate_var",
-``∀s env vn res. Cevaluate s env (CVar vn) res = (vn < LENGTH env ∧ (res = (s, Cval (EL vn env))))``,
+``∀menv s env vn res. Cevaluate menv s env (CVar (Short vn)) res = (vn < LENGTH env ∧ (res = (s, Cval (EL vn env))))``,
 rw[Once Cevaluate_cases] >> PROVE_TAC[])
 
 val _ = export_rewrites["Cevaluate_lit","Cevaluate_var"]
 
 val Cevaluate_con = store_thm(
 "Cevaluate_con",
-``∀s env cn es res. Cevaluate s env (CCon cn es) res ⇔
-(∃s' vs. Cevaluate_list s env es (s', Cval vs) ∧ (res = (s', Cval (CConv cn vs)))) ∨
-(∃s' err. Cevaluate_list s env es (s', Cexc err) ∧ (res = (s', Cexc err)))``,
+``∀menv s env cn es res. Cevaluate menv s env (CCon cn es) res ⇔
+(∃s' vs. Cevaluate_list menv s env es (s', Cval vs) ∧ (res = (s', Cval (CConv cn vs)))) ∨
+(∃s' err. Cevaluate_list menv s env es (s', Cexc err) ∧ (res = (s', Cexc err)))``,
 rw[Once Cevaluate_cases] >> PROVE_TAC[])
 
 val Cevaluate_tageq = store_thm(
 "Cevaluate_tageq",
-``∀s env exp n res. Cevaluate s env (CTagEq exp n) res ⇔
-  (∃s' m vs. Cevaluate s env exp (s', Cval (CConv m vs)) ∧ (res = (s', Cval (CLitv (Bool (n = m)))))) ∨
-  (∃s' err. Cevaluate s env exp (s', Cexc err) ∧ (res = (s', Cexc err)))``,
+``∀menv s env exp n res. Cevaluate menv s env (CTagEq exp n) res ⇔
+  (∃s' m vs. Cevaluate menv s env exp (s', Cval (CConv m vs)) ∧ (res = (s', Cval (CLitv (Bool (n = m)))))) ∨
+  (∃s' err. Cevaluate menv s env exp (s', Cexc err) ∧ (res = (s', Cexc err)))``,
 rw[Once Cevaluate_cases] >> PROVE_TAC[])
 
 val Cevaluate_let = store_thm(
 "Cevaluate_let",
-``∀s env e b res. Cevaluate s env (CLet e b) res ⇔
-(∃s' v. Cevaluate s env e (s', Cval v) ∧
-     Cevaluate s' (v::env) b res) ∨
-(∃s' err. Cevaluate s env e (s', Cexc err) ∧ (res = (s', Cexc err)))``,
+``∀menv s env e b res. Cevaluate menv s env (CLet e b) res ⇔
+(∃s' v. Cevaluate menv s env e (s', Cval v) ∧
+     Cevaluate menv s' (v::env) b res) ∨
+(∃s' err. Cevaluate menv s env e (s', Cexc err) ∧ (res = (s', Cexc err)))``,
 rw[Once Cevaluate_cases] >> PROVE_TAC[])
 
 val Cevaluate_proj = store_thm(
 "Cevaluate_proj",
-``∀s env exp n res. Cevaluate s env (CProj exp n) res ⇔
-  (∃s' m vs. Cevaluate s env exp (s', Cval (CConv m vs)) ∧ (n < LENGTH vs) ∧ (res = (s', Cval (EL n vs)))) ∨
-  (∃s' err. Cevaluate s env exp (s', Cexc err) ∧ (res = (s', Cexc err)))``,
+``∀menv s env exp n res. Cevaluate menv s env (CProj exp n) res ⇔
+  (∃s' m vs. Cevaluate menv s env exp (s', Cval (CConv m vs)) ∧ (n < LENGTH vs) ∧ (res = (s', Cval (EL n vs)))) ∨
+  (∃s' err. Cevaluate menv s env exp (s', Cexc err) ∧ (res = (s', Cexc err)))``,
 rw[Once Cevaluate_cases] >> PROVE_TAC[])
 
 (* syneq equivalence relation lemmas *)
@@ -636,7 +641,8 @@ val syneq_exp_refl = store_thm("syneq_exp_refl",
     Cases >> srw_tac[ARITH_ss][] ) >>
   strip_tac >- (
     rw[Once syneq_exp_cases] >>
-    Cases_on`n < z` >> fsrw_tac[ARITH_ss][] ) >>
+    Cases_on`i`>>fs[]>>
+    Cases_on`a < z` >> fsrw_tac[ARITH_ss][] ) >>
   strip_tac >- rw[Once syneq_exp_cases] >>
   strip_tac >- (
     rw[] >> rw[Once syneq_exp_cases] >>
@@ -809,6 +815,7 @@ val syneq_exp_sym_no_labs = store_thm("syneq_exp_sym_no_labs",
     fs[] >> HINT_EXISTS_TAC >>
     simp[inv_DEF] >> Cases >> simp[] ) >>
   strip_tac >- ( rw[] >> rw[Once syneq_exp_cases,inv_DEF] ) >>
+  strip_tac >- ( rw[] >> rw[Once syneq_exp_cases,inv_DEF] ) >>
   strip_tac >- ( rw[] >> rw[Once syneq_exp_cases] ) >>
   strip_tac >- (
     rw[] >> rw[Once syneq_exp_cases] >>
@@ -916,6 +923,10 @@ val syneq_exp_trans = store_thm("syneq_exp_trans",
     simp[O_DEF] >>
     srw_tac[DNF_ss,ARITH_ss][] >>
     metis_tac[]) >>
+  strip_tac >- (
+    rw[] >> pop_assum mp_tac >>
+    simp[Once syneq_exp_cases] >> strip_tac >>
+    simp[Once syneq_exp_cases,O_DEF] >> PROVE_TAC[]) >>
   strip_tac >- (
     rw[] >> pop_assum mp_tac >>
     simp[Once syneq_exp_cases] >> strip_tac >>
@@ -1151,7 +1162,7 @@ val good_cmap_def = Define`
       ((FAPPLY m (FST p1) = FAPPLY m (FST p2)) ⇒ (p1 = p2))`
 
 val Cevaluate_list_LENGTH = store_thm("Cevaluate_list_LENGTH",
-  ``∀exps s env s' vs. Cevaluate_list s env exps (s', Cval vs) ⇒ (LENGTH vs = LENGTH exps)``,
+  ``∀exps menv s env s' vs. Cevaluate_list menv s env exps (s', Cval vs) ⇒ (LENGTH vs = LENGTH exps)``,
   Induct >> rw[LENGTH_NIL] >> pop_assum mp_tac >>
   rw[Once Cevaluate_cases] >>
   fsrw_tac[DNF_ss][] >>
@@ -1166,8 +1177,8 @@ val MAP_SND_free_labs_any_ez = store_thm("MAP_SND_free_labs_any_ez",
   ho_match_mp_tac free_labs_ind >> rw[] >> metis_tac[])
 
 val Cevaluate_store_SUBSET = store_thm("Cevaluate_store_SUBSET",
-  ``(∀s env exp res. Cevaluate s env exp res ⇒ LENGTH s ≤ LENGTH (FST res)) ∧
-    (∀s env exps res. Cevaluate_list s env exps res ⇒ LENGTH s ≤ LENGTH (FST res))``,
+  ``(∀menv s env exp res. Cevaluate menv s env exp res ⇒ LENGTH s ≤ LENGTH (FST res)) ∧
+    (∀menv s env exps res. Cevaluate_list menv s env exps res ⇒ LENGTH s ≤ LENGTH (FST res))``,
   ho_match_mp_tac Cevaluate_ind >> rw[] >>
   TRY (PROVE_TAC [LESS_EQ_TRANS]) >- (
     Cases_on`uop`>>rw[]>>srw_tac[ARITH_ss][] >>
@@ -1192,14 +1203,16 @@ val CevalPrim2_Clocs = store_thm("CevaluatePrim2_Clocs",
   Cases >> fs[] >> rw[] >> rw[])
 
 val Cevaluate_Clocs = store_thm("Cevaluate_Clocs",
-  ``(∀s env exp res. Cevaluate s env exp res ⇒
+  ``(∀menv s env exp res. Cevaluate menv s env exp res ⇒
+     BIGUNION (IMAGE (BIGUNION o IMAGE all_Clocs o set) (FRANGE menv)) ⊆ count (LENGTH s) ∧
      BIGUNION (IMAGE all_Clocs (set env)) ⊆ count (LENGTH s) ∧
      BIGUNION (IMAGE all_Clocs (set s)) ⊆ count (LENGTH s)
      ⇒
      BIGUNION (IMAGE all_Clocs (set (FST res))) ⊆ count (LENGTH (FST res)) ∧
      (∀v. (SND res = Cval v) ⇒ all_Clocs v ⊆ count (LENGTH (FST res))) ∧
      (∀v. (SND res = Cexc (Craise v)) ⇒ all_Clocs v ⊆ count (LENGTH (FST res)))) ∧
-    (∀s env exps res. Cevaluate_list s env exps res ⇒
+    (∀menv s env exps res. Cevaluate_list menv s env exps res ⇒
+     BIGUNION (IMAGE (BIGUNION o IMAGE all_Clocs o set) (FRANGE menv)) ⊆ count (LENGTH s) ∧
      BIGUNION (IMAGE all_Clocs (set env)) ⊆ count (LENGTH s) ∧
      BIGUNION (IMAGE all_Clocs (set s)) ⊆ count (LENGTH s)
      ⇒
@@ -1221,6 +1234,10 @@ val Cevaluate_Clocs = store_thm("Cevaluate_Clocs",
   strip_tac >- (
     rw[] >>
     fsrw_tac[DNF_ss][SUBSET_DEF,MEM_EL] >>
+    PROVE_TAC[] ) >>
+  strip_tac >- (
+    rw[] >>
+    fsrw_tac[DNF_ss][SUBSET_DEF,MEM_EL,IN_FRANGE,FLOOKUP_DEF] >>
     PROVE_TAC[] ) >>
   strip_tac >- rw[] >>
   strip_tac >- srw_tac[ETA_ss][] >>
@@ -1249,18 +1266,26 @@ val Cevaluate_Clocs = store_thm("Cevaluate_Clocs",
     rpt gen_tac >> ntac 2 strip_tac >>
     fs[] >> rfs[] >>
     first_x_assum match_mp_tac >>
-    fsrw_tac[DNF_ss][SUBSET_DEF] >>
+    imp_res_tac Cevaluate_store_SUBSET >>
+    conj_tac >- (
+      match_mp_tac SUBSET_TRANS >>
+      qexists_tac`count (LENGTH s)` >>
+      simp[] >> simp[SUBSET_DEF] >>
+      fs[] >> simp[] ) >>
+    qpat_assum`P ⇒ Q`mp_tac >>
+    discharge_hyps >- (
+      fsrw_tac[DNF_ss][SUBSET_DEF] >>
+      metis_tac[LESS_LESS_EQ_TRANS] ) >>
+    simp[] >> strip_tac >>
     PairCases_on`def`>>Cases_on`def0`>>fs[LET_THM] >- (
+      fsrw_tac[DNF_ss][SUBSET_DEF] >>
       fsrw_tac[DNF_ss][MEM_GENLIST]>>
-      imp_res_tac Cevaluate_store_SUBSET >>
       fs[] >> metis_tac[LESS_LESS_EQ_TRANS] ) >>
+    fsrw_tac[DNF_ss][SUBSET_DEF] >>
     PairCases_on`x`>>
     fsrw_tac[DNF_ss][MEM_MAP,IN_FRANGE,UNCURRY] >>
     rfs[] >>
-    imp_res_tac Cevaluate_store_SUBSET >>
     fsrw_tac[ARITH_ss][] >>
-    reverse conj_tac >- metis_tac[LESS_LESS_EQ_TRANS] >>
-    conj_tac >- metis_tac[LESS_LESS_EQ_TRANS] >>
     fsrw_tac[DNF_ss][EVERY_MEM,MEM_EL] >>
     metis_tac[LESS_LESS_EQ_TRANS]) >>
   strip_tac >- (
@@ -1284,7 +1309,7 @@ val Cevaluate_Clocs = store_thm("Cevaluate_Clocs",
     rw[] >> imp_res_tac CevalPrim2_Clocs >> rw[] ) >>
   strip_tac >- rw[] >>
   strip_tac >- (
-    ntac 5 gen_tac >>
+    ntac 6 gen_tac >>
     Cases >> fs[] >>
     gen_tac >> ntac 2 strip_tac >>
     fs[] >>
@@ -1303,12 +1328,24 @@ val Cevaluate_Clocs = store_thm("Cevaluate_Clocs",
   strip_tac >- (
     rpt gen_tac >> ntac 2 strip_tac >>
     fs[] >> rfs[] >>
+    qpat_assum`P ⇒ Q`mp_tac >>
+    imp_res_tac Cevaluate_store_SUBSET >>
+    discharge_hyps >- (
+      fsrw_tac[DNF_ss][SUBSET_DEF] >>
+      metis_tac[LESS_LESS_EQ_TRANS] ) >>
+    simp[] >> strip_tac >>
     fsrw_tac[DNF_ss][SUBSET_DEF] >>
-    metis_tac[Cevaluate_store_SUBSET,LESS_LESS_EQ_TRANS,FST]) >>
+    metis_tac[LESS_LESS_EQ_TRANS]) >>
   strip_tac >- rw[] >>
   rw[] >> fs[] >> rfs[] >>
+  imp_res_tac Cevaluate_store_SUBSET >>
+  qpat_assum`P ⇒ Q`mp_tac >>
+  discharge_hyps >- (
+    fsrw_tac[DNF_ss][SUBSET_DEF] >>
+    metis_tac[LESS_LESS_EQ_TRANS] ) >>
+  simp[] >> strip_tac >>
   fsrw_tac[DNF_ss][SUBSET_DEF] >>
-  metis_tac[Cevaluate_store_SUBSET,LESS_LESS_EQ_TRANS,FST])
+  metis_tac[LESS_LESS_EQ_TRANS])
 
 (* simple cases of syneq preservation *)
 
